theories/common.v
@@ -1,0 +1,47 @@
+Require Import Lists.List.
+Require Import Lia.
+
+
+(** Definition of [lastn n l]: gives the last [n] elements of a list [l]. *)
+Definition lastn {A} n (l: list A) := List.skipn ((List.length l) - n) l.
+
+Theorem lastn_def_lastn {A} n (l: list A):
+  lastn n l = List.skipn ((List.length l) - n) l.
+Proof.
+  eauto.
+Qed.
+
+Theorem lastn_def_firstn {A} n (l: list A):
+  lastn n l = rev (firstn n (rev l)).
+Proof.
+  rewrite firstn_rev.
+  rewrite rev_involutive.
+  eauto.
+Qed.
+
+(* Some properties about [lastn]. *)
+Lemma length_lastn {A} n:
+  forall l: list A, List.length (lastn n l) = min n (List.length l).
+Proof.
+  unfold lastn.
+  setoid_rewrite List.skipn_length; lia.
+Qed.
+
+Lemma lastn_cons {A} n:
+  forall a (l: list A), length l >= n -> lastn n (a::l) = lastn n l.
+Proof.
+  unfold lastn.
+  intros.
+  simpl length.
+  replace (S (length l) - n) with (S (length l - n)); eauto.
+  lia.
+Qed.
+
+Lemma lastn_length {A}:
+  forall (a: A) l, lastn (length l) (a :: l) = l.
+Proof.
+  intros.
+  rewrite lastn_def_lastn.
+  replace (length (a :: l) - length l) with 1 by (simpl length; lia).
+  simpl; eauto.
+Qed.
